Stlc/Value.lean
@@ -1,0 +1,31 @@
+import Mathlib.Tactic.Common
+import Stlc.Syntax
+
+namespace Stlc.Term
+
+open Syntax
+
+@[mk_iff]
+inductive Value : Term → Prop
+| abs {x τ t} : Value t[λ x : τ, t]
+| true : Value t[true]
+| false : Value t[false]
+
+attribute [simp] Value.abs Value.true Value.false
+
+@[simp]
+lemma Value.var_not {x : String} : ¬Value (var x) := by
+  rintro ⟨⟩
+
+@[simp]
+lemma Value.app_not {t₁ t₂ : Term} : ¬Value t[t₁ t₂] := by
+  rintro ⟨⟩
+
+@[simp]
+lemma Value.ite_not {t₁ t₂ t₃ : Term} : ¬Value t[if t₁ then t₂ else t₃] := by
+  rintro ⟨⟩
+
+instance : DecidablePred Value := fun t ↦
+  decidable_of_bool (t matches .true | .false | .abs ..) (by cases t <;> simp)
+
+end Stlc.Term
